Pass WIP

Iris/Iris/Algebra/Lib/ExclAuth.lean
@@ -9,6 +9,8 @@ public import Iris.Algebra.Auth
 public import Iris.Algebra.Excl
 meta import Iris.Std.RocqPorting
 
+public section
+
 /-!
 # Exclusive Authoritative CMRA
 
@@ -26,92 +28,92 @@ namespace ExclAuth
 variable [OFE A]
 
 @[rocq_alias excl_authR]
-public abbrev ExclAuthR := Auth (Option (Excl A))
+abbrev ExclAuthR := Auth (Option (Excl A))
 
 @[rocq_alias excl_authUR]
-public abbrev ExclAuthUR := Auth (Option (Excl A))
+abbrev ExclAuthUR := Auth (Option (Excl A))
 
 @[rocq_alias excl_auth_auth]
-public abbrev auth (a : A) : ExclAuthR (A := A) := ● (some (excl a))
+abbrev auth (a : A) : ExclAuthR (A := A) := ● (some (excl a))
 
 @[rocq_alias excl_auth_frag]
-public abbrev frag (a : A) : ExclAuthR (A := A) := ◯ (some (excl a))
+abbrev frag (a : A) : ExclAuthR (A := A) := ◯ (some (excl a))
 
 scoped notation "●E " a => ExclAuth.auth a
 scoped notation "◯E " a => ExclAuth.frag a
 
 @[rocq_alias excl_auth_auth_ne]
-public instance auth_ne : NonExpansive (auth (A := A)) where
+instance auth_ne : NonExpansive (auth (A := A)) where
   ne _ _ _ h := Auth.auth_ne.ne (some_dist_some.mpr h)
 
 #rocq_ignore excl_auth_auth_proper "Derivable from auth_ne with NonExpansive.eqv"
 
 @[rocq_alias excl_auth_frag_ne]
-public instance frag_ne : NonExpansive (frag (A := A)) where
+instance frag_ne : NonExpansive (frag (A := A)) where
   ne _ _ _ h := Auth.frag_ne.ne (some_dist_some.mpr h)
 #rocq_ignore excl_auth_frag_proper "Derivable from frag_ne with NonExpansive.eqv"
 
 @[rocq_alias excl_auth_auth_discrete]
-public instance auth_discrete {a : A} [DiscreteE a] : DiscreteE (●E a) :=
+instance auth_discrete {a : A} [DiscreteE a] : DiscreteE (●E a) :=
   letI _ : DiscreteE (some (excl a)) := some_is_discrete
   letI _ : DiscreteE (unit : Option (Excl A)) := none_is_discrete
   by infer_instance
 
 @[rocq_alias excl_auth_frag_discrete]
-public instance frag_discrete {a : A} [DiscreteE a] : DiscreteE (◯E a) :=
+instance frag_discrete {a : A} [DiscreteE a] : DiscreteE (◯E a) :=
   letI _ : DiscreteE (some (excl a)) := some_is_discrete
   by infer_instance
 
 @[rocq_alias excl_auth_validN]
-public theorem validN {a : A} : ✓{n} (●E a) • ◯E a :=
+theorem validN {a : A} : ✓{n} (●E a) • ◯E a :=
   Auth.both_validN.mpr ⟨.rfl, trivial⟩
 
 @[rocq_alias excl_auth_valid]
-public theorem valid {a : A} : ✓ (●E a) • ◯E a :=
+theorem valid {a : A} : ✓ (●E a) • ◯E a :=
   Auth.auth_both_valid_2 trivial .rfl
 
 @[rocq_alias excl_auth_agreeN]
-public theorem agreeN {a b : A} (h : ✓{n} (●E a) • ◯E b) : a ≡{n}≡ b :=
+theorem agreeN {a b : A} (h : ✓{n} (●E a) • ◯E b) : a ≡{n}≡ b :=
   dist_of_inc_exclusive (Auth.both_validN.mp h).1 trivial |>.symm
 
 @[rocq_alias excl_auth_agree]
-public theorem agree {a b : A} (h : ✓ (●E a) • ◯E b) : a ≡ b :=
+theorem agree {a b : A} (h : ✓ (●E a) • ◯E b) : a ≡ b :=
   equiv_dist.mpr fun _ => agreeN (Valid.validN h)
 
 @[rocq_alias excl_auth_agree_L]
-public theorem agree_L [Leibniz A] {a b : A} (h : ✓ (●E a) • ◯E b) : a = b :=
+theorem agree_L [Leibniz A] {a b : A} (h : ✓ (●E a) • ◯E b) : a = b :=
   (agree h).to_eq
 
 @[rocq_alias excl_auth_auth_op_validN]
-public theorem auth_op_validN {a b : A} : (✓{n} (●E a) • ●E b) ↔ False :=
+theorem auth_op_validN {a b : A} : (✓{n} (●E a) • ●E b) ↔ False :=
   Auth.auth_op_validN
 
 @[rocq_alias excl_auth_auth_op_valid]
-public theorem auth_op_valid {a b : A} : (✓ (●E a) • ●E b) ↔ False :=
+theorem auth_op_valid {a b : A} : (✓ (●E a) • ●E b) ↔ False :=
   Auth.auth_op_valid
 
 @[rocq_alias excl_auth_frag_op_validN]
-public theorem frag_op_validN {a b : A} : (✓{n} (◯E a) • ◯E b) ↔ False := by
+theorem frag_op_validN {a b : A} : (✓{n} (◯E a) • ◯E b) ↔ False := by
   suffices H : ✓{n} some (excl a) • some (excl b) ↔ False by rwa [Auth.frag_op.symm, Auth.frag_validN]
   exact ⟨not_valid_some_exclN_op_left, False.elim⟩
 
 @[rocq_alias excl_auth_frag_op_valid]
-public theorem frag_op_valid {a b : A} : (✓ (◯E a) • ◯E b) ↔ False := by
+theorem frag_op_valid {a b : A} : (✓ (◯E a) • ◯E b) ↔ False := by
   suffices H : ✓ some (excl a) • some (excl b) ↔ False by rwa [Auth.frag_op.symm, Auth.frag_valid]
   exact ⟨fun h => not_valid_some_exclN_op_left (n := 0) h.validN, False.elim⟩
 
 @[rocq_alias excl_auth_update]
-public theorem update {a b a' : A} : ((●E a) • ◯E b) ~~> ((●E a') • ◯E a') :=
+theorem update {a b a' : A} : ((●E a) • ◯E b) ~~> ((●E a') • ◯E a') :=
   Auth.auth_update (.option (.exclusive trivial))
 
 /-! ## Functors -/
 
 @[rocq_alias excl_authURF]
-public abbrev ExclAuthURF (T : COFE.OFunctorPre) [URFunctor T] : COFE.OFunctorPre :=
+abbrev ExclAuthURF (T : COFE.OFunctorPre) [URFunctor T] : COFE.OFunctorPre :=
   AuthURF (OptionOF (ExclOF T))
 
 @[rocq_alias excl_authRF]
-public abbrev ExclAuthRF (T : COFE.OFunctorPre) [URFunctor T] : COFE.OFunctorPre :=
+abbrev ExclAuthRF (T : COFE.OFunctorPre) [URFunctor T] : COFE.OFunctorPre :=
   AuthRF (OptionOF (ExclOF T))
 
 end ExclAuth
