Iris/Iris/BI/Algebra.lean
@@ -31,13 +31,11 @@ theorem prod_validI [Sbi PROP] [CMRA A] [CMRA B] (x : A × B) :
 theorem prod_includedI [Sbi PROP] [CMRA A] [CMRA B] (x y : A × B) :
     internalCmraIncluded x y ⊣⊢@{PROP} internalCmraIncluded x.1 y.1 ∧ internalCmraIncluded x.2 y.2 := by
   simp only [internalCmraIncluded,  internalEq]
-  refine .trans ?_ siPure_and
-  refine siPure_mono_bi ?_
+  refine .trans (siPure_mono_bi ?_) siPure_and
   refine siPure_exist.symm.trans ?_
   refine .trans ?_ (and_congr_left siPure_exist)
   refine .trans ?_ (and_congr_right siPure_exist)
-  refine .trans ?_ siPure_and
-  refine siPure_mono_bi ?_
+  refine .trans (siPure_mono_bi ?_) siPure_and
   cases x with | mk x1 x2 =>
   cases y with | mk y1 y2 =>
   simp only [CMRA.op, Prod.op]
@@ -73,11 +71,9 @@ theorem option_includedI [Sbi PROP] [CMRA A] {mx my : Option A} :
   · refine ⟨?_, false_elim⟩
     refine .trans (siPure_mono ?_) siPure_pure.mp
     rintro n ⟨_, ⟨c, rfl⟩, hc⟩
-    rcases c with _ | c <;>
-      exact (hc : False)
+    rcases c with _ | c <;> exact hc
   · simp only [internalCmraIncluded, internalEq]
-    refine .trans ?_ siPure_or
-    refine siPure_mono_bi ⟨fun n h => ?_, fun n h => ?_⟩
+    refine .trans (siPure_mono_bi ⟨fun n h => ?_, fun n h => ?_⟩) siPure_or
     · obtain ⟨_, ⟨c, rfl⟩, hc⟩ := h
       rcases Option.some_incN_some_iff.mp ⟨c, hc⟩ with heqv | ⟨c, hc⟩
       · exact .inr heqv
@@ -101,8 +97,7 @@ theorem option_included_totalI [Sbi PROP] [CMRA A] [CMRA.IsTotal A] {mx my : Opt
   · refine ⟨?_, false_elim⟩
     refine .trans (siPure_mono ?_) siPure_pure.mp
     rintro n ⟨_, ⟨c, rfl⟩, hc⟩
-    rcases c with _ | c <;>
-      exact (hc : False)
+    rcases c with _ | c <;> exact hc
   · refine siPure_mono_bi ⟨fun n h => ?_, fun n h => ?_⟩
     · obtain ⟨_, ⟨c, rfl⟩, hc⟩ := h
       obtain ⟨c, hc⟩ := Option.some_incN_some_iff_is_total.mp ⟨c, hc⟩
@@ -227,13 +222,13 @@ open Iris BI Agree OFE
 variable [Sbi PROP] [OFE A]
 
 @[rocq_alias agree_equivI]
-theorem agree_equivI (a b : A) : internalEq (toAgree a) (toAgree b) ⊣⊢@{PROP} internalEq a b := by
+theorem agree_equivI {a b : A} : internalEq (toAgree a) (toAgree b) ⊣⊢@{PROP} internalEq a b := by
   refine ⟨siPure_mono fun _ => Agree.toAgree_injN, ?_⟩
   refine siPure_mono fun n => ?_
   apply NonExpansive.ne
 
 @[rocq_alias agree_op_invI]
-theorem agree_op_invI (x y : Agree A) : internalCmraValid (x • y) ⊢@{PROP} internalEq x y :=
+theorem agree_op_invI {x y : Agree A} : internalCmraValid (x • y) ⊢@{PROP} internalEq x y :=
   siPure_mono (fun _ => op_invN)
 
 @[rocq_alias to_agree_validI]
@@ -266,7 +261,7 @@ theorem agree_op_equiv_toAgreeI (x y : Agree A) (a : A) :
   have H1 : internalEq (x • y) (toAgree a) ⊢@{PROP} internalEq x y := by
     refine absorbingly_internalEq (x • y) (toAgree a) |>.mpr.trans ?_
     refine (absorbingly_mono ?_).trans absorbing
-    refine internalEq.rewrite' internalCmraValid internalEq.symm ?_ |>.trans (agree_op_invI x y)
+    refine internalEq.rewrite' internalCmraValid internalEq.symm ?_ |>.trans agree_op_invI
     refine emp_sep.2.trans ?_
     refine (sep_mono_left (toAgree_validI a)) |>.trans ?_
     exact sep_elim_left
