Iris/Iris/BI/DerivedLawsLater.lean
@@ -403,7 +403,7 @@ instance laterN_persistent (n : Nat) (P : PROP) [Persistent P] :
   | zero => assumption
   | succ n _ => exact later_persistent
 
-instance laterIf_persistent [BI PROP] (P : PROP) [Persistent P] (p : Bool) :
+instance instPersistentLaterIf [BI PROP] (P : PROP) [Persistent P] (p : Bool) :
     Persistent iprop(▷?p P) := by
   cases p <;> simp [BIBase.laterIf] <;> infer_instance
 
